foundations complete,ready to prove

LeanCCS/LabelledTransitionSystem.lean
@@ -10,14 +10,33 @@ instance : LawfulBEq State where
   rfl := by simp [State.beq_iff]
   eq_of_beq h := State.ext _ _ (State.beq_iff.1 h)
 
+@[ext]
 structure Action where
   val : String
+deriving BEq
+
+theorem Action.beq_iff {a b : Action} : (a == b) ↔ a.val = b.val := by
+  rw [show a == b ↔ a.val == b.val from Iff.rfl, beq_iff_eq]
+
+instance : LawfulBEq Action where
+  rfl := by simp [Action.beq_iff]
+  eq_of_beq h := Action.ext _ _ (Action.beq_iff.1 h)
 
 structure LTS where
   states : List State
   actions : List Action
-  transition : State → Action → List { s : State // s ∈ states }
-  s0 : State
+  transition : { s : State // s ∈ states } → { a : Action // a ∈ actions } → List { s : State // s ∈ states }
+  s0 : { s : State // s ∈ states }
 
 def map_lts_statesList (lts : LTS) : List { s : State // s ∈ lts.states } :=
   lts.states.filterMap fun s ↦ if h : s ∈ lts.states then some ⟨s, h⟩ else none
+
+def map_lts_actionsList (lts : LTS) : List { a : Action // a ∈ lts.actions } :=
+  lts.actions.filterMap fun a ↦ if h : a ∈ lts.actions then some ⟨a, h⟩ else none
+
+-- Main theorem
+theorem reach_iff_pre_star {lts : LTS}
+  (s : { s : State // s ∈ lts.states })
+  (s' : { s : State // s ∈ lts.states }) :
+  s'.val ∈ reach [s] ↔ s.val ∈ pre_star [s'] := by
+  sorry
