LeanCCS/Post.lean
@@ -3,19 +3,19 @@ import LeanCCS.Utils
 
 open List
 
-protected def LTS.post {lts : LTS} (s : { s : State // s ∈ lts.states }) (a : Action) : List { s : State // s ∈ lts.states } :=
+def post {lts : LTS} (s : { s : State // s ∈ lts.states }) (a : {a : Action // a ∈ lts.actions }) : List { s : State // s ∈ lts.states } :=
   lts.transition s a
 
-def post_S {lts : LTS} (states : List { s : State // s ∈ lts.states }) (a : Action) : List { s : State // s ∈ lts.states } :=
-  states.foldl (fun acc state => acc ++ lts.post state a) []
+def post_S {lts : LTS} (states : List { s : State // s ∈ lts.states }) (a : { a : Action // a ∈ lts.actions }) : List { s : State // s ∈ lts.states } :=
+  states.foldl (fun acc state => acc ++ post state a) []
 
-def post_A {lts : LTS} (s : { s : State // s ∈ lts.states }) (actions : List Action) : List { s : State // s ∈ lts.states } :=
-  actions.foldl (fun acc act => acc ++ lts.post s act) []
+def post_A {lts : LTS} (s : { s : State // s ∈ lts.states }) (actions : List { a : Action // a ∈ lts.actions }) : List { s : State // s ∈ lts.states } :=
+  actions.foldl (fun acc act => acc ++ post s act) []
 
-def post_S_A {lts : LTS} (states : List { s : State // s ∈ lts.states }) (actions : List Action) : List { s : State // s ∈ lts.states } :=
+def post_S_A {lts : LTS} (states : List { s : State // s ∈ lts.states }) (actions : List { a : Action // a ∈ lts.actions }) : List { s : State // s ∈ lts.states } :=
   actions.foldl (fun acc act => acc ++ post_S states act) []
 
-def post_S_n {lts : LTS} (states : List { s : State // s ∈ lts.states }) (actions : List Action) (n : Nat) : List { s : State // s ∈ lts.states } :=
+def post_S_n {lts : LTS} (states : List { s : State // s ∈ lts.states }) (actions : List { a : Action // a ∈ lts.actions }) (n : Nat) : List { s : State // s ∈ lts.states } :=
   match n with
   | 0 => states
   | n' + 1 => post_S_A (post_S_n states actions n') actions
@@ -35,8 +35,16 @@ def reach_aux (lts : LTS) (visited : { l : List State // l <+~ lts.states } )
       have : lts.states.length - (visited.1.length + 1) < lts.states.length - visited.1.length := by
         refine Nat.sub_add_lt_sub ?_ Nat.zero_lt_one
         simpa using hx.length_le
-      reach_aux lts ⟨s::visited, hx⟩ (  (post_A  s lts.actions)  ++ ss) ( (post_A  s lts.actions).map Subtype.val ++ acc )
+      let actions_with_proof := map_lts_actionsList lts
+      reach_aux lts ⟨s::visited, hx⟩ (post_A s actions_with_proof ++ ss) ((post_A s actions_with_proof).map Subtype.val ++ acc)
 termination_by (lts.states.length - visited.1.length, to_visit.length)
 
 def reach {lts : LTS} (initial_states : List { s : State // s ∈ lts.states }) : List State :=
   reach_aux lts ⟨[], nil_subperm⟩ initial_states []
+
+theorem post_S_n_succ_eq_post_S_n_post_S_n {lts : LTS}
+  (states : List { s : State // s ∈ lts.states })
+  (actions : List { a : Action // a ∈ lts.actions })
+  (n : Nat) :
+  post_S_n states actions (n + 1) = post_S_n (post_S_n states actions n) actions 1 := by
+  rfl
