LeanCCS/Pre.lean
@@ -8,10 +8,12 @@ local instance instBEqSubtype {α : Type _} [BEq α] (P: α → Prop) : BEq (Sub
 
 local instance {lts : LTS} : BEq { s : State // s ∈ lts.states } := instBEqSubtype _
 
-def pre {lts : LTS} (s : { s : State // s ∈ lts.states }) (a : Action) : List { s : State // s ∈ lts.states } :=
-  List.filter (fun st => (lts.transition st a).indexOf? s != none) <| map_lts_statesList lts
+-- Pre function
+def pre {lts : LTS} (s : { s : State // s ∈ lts.states }) (a : { a : Action // a ∈ lts.actions }) : List { s : State // s ∈ lts.states } :=
+  List.filter (fun st => (lts.transition st a).indexOf? s != none) (map_lts_statesList lts)
 
-def pre_A (lts : LTS) (s : State) (actions : List Action) : List State :=
+-- Pre_A function
+def pre_A (lts : LTS) (s : State) (actions : List { a : Action // a ∈ lts.actions }) : List State :=
   let s_subtype : Option { s : State // s ∈ lts.states } :=
     if h : s ∈ lts.states then some ⟨s, h⟩ else none
   match s_subtype with
@@ -19,7 +21,8 @@ def pre_A (lts : LTS) (s : State) (actions : List Action) : List State :=
   | some s' =>
     actions.foldl (fun acc a => acc ++ (pre s' a).map Subtype.val) []
 
-def pre_S (lts : LTS) (states : List State) (a : Action) : List State :=
+-- Pre_S function
+def pre_S (lts : LTS) (states : List State) (a : { a : Action // a ∈ lts.actions }) : List State :=
   states.foldl (fun acc s =>
     let s_subtype : Option { s : State // s ∈ lts.states } :=
       if h : s ∈ lts.states then some ⟨s, h⟩ else none
@@ -28,10 +31,36 @@ def pre_S (lts : LTS) (states : List State) (a : Action) : List State :=
     | some s' => acc ++ (pre s' a).map Subtype.val
   ) []
 
-def pre_S_A (lts : LTS) (states : List State) (actions : List Action) : List State :=
+-- Pre_S_A function
+def pre_S_A (lts : LTS) (states : List State) (actions : List { a : Action // a ∈ lts.actions }) : List State :=
   actions.foldl (fun acc action => acc ++ pre_S lts states action) []
 
-def pre_S_n (lts : LTS) (states : List State) (actions : List Action) (n : Nat) : List State :=
+-- Pre_S_n function
+def pre_S_n (lts : LTS) (states : List State) (actions : List { a : Action // a ∈ lts.actions }) (n : Nat) : List State :=
   match n with
   | 0 => states
   | n' + 1 => pre_S_A lts (pre_S_n lts states actions n') actions
+
+
+def pre_star_aux (lts : LTS) (visited : { l : List State // l <+~ lts.states })
+(to_visit : List { s : State // s ∈ lts.states }) (acc : List State) : List State :=
+  match to_visit with
+  | [] => acc
+  | s::ss =>
+    if h : visited.1.indexOf? s.1 != none then
+      pre_star_aux lts visited ss acc
+    else
+      have hx : (s.1 :: visited.1) <+~ lts.states := by
+        refine List.cons_subperm_of_not_mem_of_mem ?_ s.2 visited.2
+        rw [Bool.not_eq_true, bne_eq_false_iff_eq] at h
+        exact List.not_mem_of_indexOf?_eq_none _ _ h
+      have : lts.states.length - (visited.1.length + 1) < lts.states.length - visited.1.length := by
+        refine Nat.sub_add_lt_sub ?_ Nat.zero_lt_one
+        simpa using hx.length_le
+      let actions_with_proof := map_lts_actionsList lts
+      let predecessors := actions_with_proof.foldl (fun acc a => acc ++ pre s a) []
+      pre_star_aux lts ⟨s.1::visited.1, hx⟩ (predecessors ++ ss) (s.1 :: acc)
+termination_by (lts.states.length - visited.1.length, to_visit.length)
+
+def pre_star {lts : LTS} (initial_states : List { s : State // s ∈ lts.states }) : List State :=
+  pre_star_aux lts ⟨[], nil_subperm⟩ initial_states []
